\documentclass[10pt]{jsarticle}
\bibliographystyle{junsrt}
\usepackage[dvipdfmx]{graphicx}
\usepackage[dvipdfmx,svgnames]{xcolor}%before tikz
\usepackage{tikz}
\usepackage{geometry}
\usepackage{amsmath,amssymb}
\usepackage{chemarrow}
\usepackage{booktabs}
\usepackage{longtable}
\usepackage{colortbl}
\usepackage{tabularx}
\usepackage{tabu}
\usepackage{float}
\usepackage{txfonts}
\usepackage{url}
\usepackage{siunitx}
\usepackage{subfigure}
\usepackage{enumerate}
\usepackage{caption}
\usepackage{wrapfig}
\usepackage{array}
\usepackage{titlesec}
\usepackage{picture}
\usepackage{multicol}
\usepackage{etoolbox}
\usepackage{fancyhdr}
% \usepackage{listings,jlisting}
% \lstset{basicstyle=\ttfamily,
%   showstringspaces=false,
%   commentstyle=\color{red},
%   keywordstyle=\color{blue}
% }
%\usepackage{makeidx}

\newcommand{\napier}{\mathrm{e}}
\newcommand{\unitone}[2]{${#1}\,\mathrm{#2}$}
\newcommand{\unittwo}[3]{${#1}\,\mathrm{#2}/\mathrm{#3}$}
\newcommand{\dif}{\mathrm{d}}
\newcommand{\bibun}[2]{\frac{\dif {#1}}{\dif {#2}}}
\newcommand{\henbibun}[2]{\frac{\partial {#1}}{\partial {#2}}}
\newcommand{\figref}[1]{図\ref{#1}}
\newcommand{\tabref}[1]{表\ref{#1}}
\renewcommand{\thesubfigure}{(\thefigure.\arabic{subfigure})}
\geometry{left=30mm, right=30mm, top=20mm, bottom=20mm}
%\makeindex

\begin{document}
% \title{}
% \author{Yutaro Konta\\Kiryu Laboratory\\Department of Computational Biology and Medical Sciences, Graduate School of Frontier Sciences, The University of Tokyo}
% %\date{}
% \maketitle
% \thispagestyle{empty}
% \newpage

%\tableofcontents
%\listoftables
%\listoffigures
\pagenumbering{arabic}

\begin{equation}
 p(D , n, t) = \prod_{k=1}^{K} \sum_{i_k} p(i_k) \sum_{h_k} p(h_k | i_k) \sum_{x_{i_k}} p(x_{i_k} | i_k, h_k, n_{i_k}, t_{i_k}, t_{\mathrm{child}(i_k)})
  \prod_{l=0}^{m_k - 1} \left( \sum_{q_{kl}} n_{q_{kl}} \frac{x_{q_{kl}}}{2} \right) \prod_{l=m_k}^{M_k - 1} \left( \sum_{q_{kl}} n_{q_{kl}} \left(1-\frac{x_{q_{kl}}}{2} \right) \right)
\end{equation}

\begin{equation}
 Z^{(k)}_{i_k, h_k, x_{i_k}, q_{k 0:(M_k - 1)}}
\end{equation}

\begin{equation}
 (t, n) = \argmax_{t, n} \ln p(D | n, t)
\end{equation}

\begin{align}
 p(D_k, z^{(k)} | n, t) &= \prod_{i_k} \prod_{h_k} \prod_{x_{i_k}} \prod_{q_{k 0:(M_k - 1)}} \Bigl\{p(i_k) p(h_k | i_k) p(x_{i_k} | i_k, h_k, n_{i_k}, t_{i_k}, t_{\mathrm{child}(i_k)})\\
&\times \prod_{l=0}^{m_k - 1} \left( n_{q_{kl}} \frac{x_{q_{kl}}}{2} \right) \prod_{l=m_k}^{M_k - 1} \left( n_{q_{kl}} \left(1-\frac{x_{q_{kl}}}{2} \right) \right) \Bigr\}^{z^{(k)}_{i_k, h_k, x_{i_k}, q_{k 0:(M_k - 1)}}}
\end{align}

\begin{align}
 \gamma(z^{(k)}_{i_k, h_k, x_{i_k}, q_{k 0:(M_k - 1)}}) &= E_{z^{(k)} | D_k, n^{\mathrm{old}}, t^{\mathrm{old}}} \left[z^{(k)}\right]\\
 &= \frac{p(i_k) p(h_k | i_k) p(x_{i_k} | i_k, h_k, n_{i_k}, t_{i_k}, t_{\mathrm{child}(i_k)}) \prod_{l=0}^{m_k - 1} \left( n_{q_{kl}} \frac{x_{q_{kl}}}{2} \right) \prod_{l=m_k}^{M_k - 1} \left( n_{q_{kl}} \left(1-\frac{x_{q_{kl}}}{2} \right) \right)}{\sum_{i_k} p(i_k) \sum_{h_k} p(h_k | i_k) \sum_{x_{i_k}} p(x_{i_k} | i_k, h_k, n_{i_k}, t_{i_k}, t_{\mathrm{child}(i_k)})
  \prod_{l=0}^{m_k - 1} \left( \sum_{q_{kl}} n_{q_{kl}} \frac{x_{q_{kl}}}{2} \right) \prod_{l=m_k}^{M_k - 1} \left( \sum_{q_{kl}} n_{q_{kl}} \left(1-\frac{x_{q_{kl}}}{2} \right) \right)}
\end{align}

\begin{align}
 Q(n,t; n^{\mathrm{old}},t^{\mathrm{old}}) &= \sum_{k=1}^{K} E_{z^{(k)} | D_k, n^{\mathrm{old}}, t^{\mathrm{old}}} \left[ \ln p(D_k ,z_k | n, t)\right]\\
 & = \sum_{k}\sum_{i_k}\sum_{h_k}\sum_{x_{i_k}} \sum_{q_{k0:(M_k-1)}} \gamma(z^{(k)})\Bigl[\ln p(i_k) + \ln p(h_k | i_k) + \ln p(x_{i_k} | i_k, h_k, n_{i_k}, t_{i_k}, t_{\mathrm{child}(i_k)})\\
 & + \sum_{l=0}^{M_k - 1} \ln n_{q_{kl}} + \sum_{l=0}^{m_k - 1} \ln \left(\frac{x_{i_{kl}}}{2}\right) + \sum_{l=m_k}^{M_k -1} \ln \left(1 - \frac{x_{i_{kl}}}{2}\right) \Bigr]
\end{align}

\begin{align}
 p(i_k) = \frac{\frac{t_{i_k}n_{i_k}}{\ln \left(N n_{i_k} \right)}}{\sum_{i=1}^{I}\frac{t_{i}n_{i}}{\ln \left(N n_{i} \right)}}
\end{align}

\begin{align}
 p(h_k | i_k) =
 \begin{cases}
  \frac{S_{i_k} - 1}{S_{i_k} + H_{i_k} - 2 - \sum_{h=1}^{H_{i_k} - 1} \frac{t_{\mathrm{eldestchild}(i_k, h)}}{t_{i_k}}} & (h_k = 0)\\
  \frac{1 - \frac{t_{\mathrm{eldestchild}(i_k, h_k)}}{t_{i_k}}}{S_{i_k} + H_{i_k} - 2 - \sum_{h=1}^{H_{i_k} - 1} \frac{t_{\mathrm{eldestchild}(i_k, h)}}{t_{i_k}}} & (h_k \neq 0)
 \end{cases}
\end{align}

\begin{align}
 \int_{0}^{t_{i_k}} \left(Nn_{i_k}(t) - 1\right) dt = t_{i_k} \left(\frac{Nn_{i_k} - 1}{\ln \left( Nn_{i_k} \right)} - 1\right)
\end{align}

\begin{align}
 \int_{t_{\mathrm{eldestchild}(i_k, h)}}^{t_{i_k}} 1 dt = t_{i_k} - t_{\mathrm{eldestchild}(i_k, h)}
\end{align}

\begin{align}
 p(h_k | i_k) =
 \begin{cases}
  \frac{\int_{0}^{t_{i_k}} \left(Nn_{i_k}(t) - 1\right) dt}{\int_{0}^{t_{i_k}} \left(Nn_{i_k}(t) - 1\right) dt + \sum_{h=1}^{H_{i_k} - 1}\int_{t_{\mathrm{eldestchild}(i_k, h)}}^{t_{i_k}} 1 dt} =  \frac{S_{i_k} - 1}{S_{i_k} + H_{i_k} - 2 - \sum_{h=1}^{H_{i_k} - 1} \frac{t_{\mathrm{eldestchild}(i_k, h)}}{t_{i_k}}} & h_k=0\\
  \frac{\int_{t_{\mathrm{eldestchild}(i_k, h_k)}}^{t_{i_k}} 1 dt}{\int_{0}^{t_{i_k}} \left(Nn_{i_k}(t) - 1\right) dt + \sum_{h=1}^{H_{i_k} - 1}\int_{t_{\mathrm{eldestchild}(i_k, h)}}^{t_{i_k}} 1 dt} = \frac{1 - \frac{t_{\mathrm{eldestchild}(i_k, h_k)}}{t_{i_k}}}{S_{i_k} + H_{i_k} - 2 - \sum_{h=1}^{H_{i_k} - 1} \frac{t_{\mathrm{eldestchild}(i_k, h)}}{t_{i_k}}} & h_k \neq 0
 \end{cases}
\end{align}

\begin{align}
 S_i = \frac{Nn_i - 1}{\ln \left( Nn_i \right)}
\end{align}

\begin{align}
 p(i_k) = \frac{\int_{0}^{t_{i_k}} \left(Nn_{i_k}(t) \right) dt}{\sum_{i=1}^{I} \int_{0}^{t_i} \left(Nn_{i}(t) \right) dt} = \frac{\frac{t_{i_k}n_{i_k}}{\ln \left(N n_{i_k} \right)}}{\sum_{i=1}^{I}\frac{t_{i}n_{i}}{\ln \left(N n_{i} \right)}}
\end{align}
%\tableofcontents
%\listoftables
%\listoffigures
\pagenumbering{arabic}

%\printindex
\end{document}


% \bibliography{}
%\printindex
\end{document}

